coqimp/ext/rellogic.v
@@ -535,9 +535,9 @@ CoInductive rel_safety : nat -> Index -> (XCodeHeap * State * Word * Word) -> (p
             exists idx1 A' HS' w ,
               ((idx1 ⩹ idx /\ A' = A /\ HS = HS') \/ (exec_prim (A, HS) (A', HS'))) /\
               (
-                (Nat.eqb k 0 = true /\ (S2, HS', A', w) ||= Q /\ A' = Pdone) \/
+                (Nat.eqb k 0 = true /\ (S2, HS', A', w) ||= Q /\ A' = Pdone /\ (0%nat, 0%nat) ⩹ idx1) \/
                 (Nat.eqb k 0 = false /\ rel_safety (Nat.pred k) idx1 (C, S2, pc2, npc2) (A', HS') Q)
-              ) /\ (0%nat, 0%nat) ⩹ idx1
+              )
       )
     ) ->
     rel_safety k idx (C, S, pc, npc) (A, HS) Q.
